impl/src/verifier/typescript_files/util.ts
@@ -55,9 +55,14 @@ function sanitizeName(name: string): string {
   // TOUPDATE: Add more `replace operations' if the IR syntax (names)
   // conflicts with FStar syntax
   let result = name
-    .replace(new RegExp("#", 'g'), "_")
+    .replace(/#/g,  "_")
+    .replace(/:/g,  "_")
+    .replace(/-/g,  "_")
+    .replace(/\//g, "_")
+    .replace(/%/g,  "_")
+    .replace(/\[/g, "_")
+    .replace(/\]/g, "_")
     .replace(new RegExp("\\$", 'g'), "_")
-    .replace(new RegExp(":", 'g'), "_")
     .replace(new RegExp("\\.", 'g'), "_")
   // We lowercase the first character because variable/function
   // declaration in fstar requires that
